Examples/CounterSpec.v
@@ -1,0 +1,24 @@
+From LHL.Core Require Import
+  Program
+  Specs.
+
+Variant CounterSig : ESig :=
+| Inc : CounterSig unit
+| Get : CounterSig nat.
+
+Variant CounterState :=
+| CounterIdle (n : nat)
+| CounterIncRunning (i : ThreadName) (n : nat)
+| CounterGetRunning (i : ThreadName) (n : nat).
+
+Variant CounterStep : CounterState -> ThreadEvent CounterSig -> CounterState -> Prop :=
+| CounterCallInc i n : CounterStep (CounterIdle n) (i, CallEv Inc) (CounterIncRunning i n)
+| CounterRetInc i n : CounterStep (CounterIncRunning i n) (i, RetEv Inc tt) (CounterIdle (S n))
+| CounterCallGet i n : CounterStep (CounterIdle n) (i, CallEv Get) (CounterGetRunning i n)
+| CounterRetGet i n : CounterStep (CounterGetRunning i n)  (i, RetEv Get n) (CounterIdle n).
+
+Definition counterSpec : Spec CounterSig := {|
+  State := CounterState;
+  Step := CounterStep;
+  Init := CounterIdle 0
+|}.
