Examples/FAISpec.v
@@ -1,0 +1,24 @@
+From LHL.Core Require Import
+  Specs
+  Traces
+  Program.
+
+From LHL.Util Require Import
+  Util.
+
+Variant FAISig : ESig :=
+| FAI : FAISig nat.
+
+Variant FAIState :=
+| FAICalled (i : ThreadName) (n : nat)
+| FAIIdle (n : nat).
+
+Variant FAIStep : FAIState -> ThreadEvent FAISig -> FAIState -> Prop :=
+| FAICall i n : FAIStep (FAIIdle n) (i, CallEv FAI) (FAICalled i n)
+| FAIRet i n : FAIStep (FAICalled i n) (i, RetEv FAI n) (FAIIdle (S n)).
+
+Definition faiSpec : Spec FAISig := {|
+  State := FAIState;
+  Step := FAIStep;
+  Init := FAIIdle 0
+|}.
