Examples/TicketLock.v
@@ -1,0 +1,60 @@
+From LHL.Core Require Import
+  Program
+  Specs
+  Logic
+  LogicFacts
+  Tensor
+  Traces
+  Linearizability.
+
+From LHL.Examples Require Import
+  LockSpec
+  FAISpec
+  YieldSpec
+  CounterSpec.
+
+From Coq Require Import
+  Arith.PeanoNat.
+
+Definition Underlay := FAISig |+| CounterSig |+| YieldSig.
+
+Definition acq : Prog Underlay unit :=
+  my_tick <- call FAI;
+  while
+    (cur_tick <- call Get; ret (negb (cur_tick =? my_tick)))
+    (call Yield).
+
+Definition rel : Prog Underlay unit :=
+  call Inc.
+
+Definition ticketLockImpl : Impl Underlay LockSig :=
+  fun _ m => match m with
+  | Acq => acq
+  | Rel => rel
+  end.
+
+Definition E := Underlay.
+Definition F := LockSig.
+Definition VE := tensorSpec faiSpec (tensorSpec counterSpec yieldSpec).
+Definition VF := lockSpec.
+
+Definition Relt := Relt VE VF.
+Definition Prec := Prec VE VF.
+Definition Post := Post VE VF.
+
+Definition Rely (i : ThreadName) : Relt :=
+  fun s ρ t σ => True.
+
+Definition Guar (i : ThreadName) : Relt :=
+  fun s ρ t σ => True.
+
+Definition Precs (i : ThreadName) {A} (m : LockSig A) : Prec :=
+  fun s ρ =>
+    True.
+
+Definition Posts (i : ThreadName) {A} (m : LockSig A) : Post A :=
+  fun _ s ρ t σ =>
+    True.
+
+Theorem ticketLockCorrect :
+  VerifyImpl VE VF Rely Guar Precs ticketLockImpl Posts.
