Examples/YieldSpec.v
@@ -1,0 +1,41 @@
+From LHL.Core Require Import
+  Specs
+  Traces
+  Program.
+
+From LHL.Util Require Import
+  Util.
+
+Variant YieldSig : ESig :=
+| Yield : YieldSig unit.
+
+Variant YieldStatus :=
+| YieldIdle
+| YieldGiving
+| YieldReceiving.
+
+Definition YieldState :=
+  ThreadName -> YieldStatus.
+
+Variant YieldStep : YieldState -> ThreadEvent YieldSig -> YieldState -> Prop :=
+| YieldCall (s t : YieldState) i :
+    s i = YieldIdle ->
+    t i = YieldGiving ->
+    (forall j, i <> j ->
+      s j = YieldGiving ->
+      t j = YieldReceiving) ->
+    (forall j, i <> j ->
+      s j = YieldReceiving \/ s j = YieldIdle ->
+      s j = t j) ->
+    YieldStep s (i, CallEv Yield) t
+| YieldRet (s t : YieldState) i :
+    s i = YieldReceiving ->
+    t i = YieldIdle ->
+    differ_pointwise s t i ->
+    YieldStep s (i, RetEv Yield tt) t.
+
+Definition yieldSpec : Spec YieldSig := {|
+  State := YieldState;
+  Step := YieldStep;
+  Init := fun _ => YieldIdle
+|}.
